UnivProof: stengthen inductive hom. for global_h

ProofLibrary/ChaseSequence.lean
@@ -204,9 +204,341 @@ namespace KnowledgeBase
     ∀ cs : ChaseSequence kb, cs.terminates
 end KnowledgeBase
 
+noncomputable def inductive_homomorphism (kb : KnowledgeBase) (cs : ChaseSequence kb) (m : FactSet) (mIsModel : m.modelsKb kb) : (i : Nat) -> { hom : GroundTermMapping // isHomomorphism hom ∧ applyFactSet hom (cs.fact_sets i) ⊆ m }
+| .zero => ⟨id, (by 
+  constructor 
+  unfold isHomomorphism ; intro gt ; cases gt <;> simp
+  rw [cs.database_first]
+  intro el 
+  simp [Set.element]
+  intro elInSet 
+  cases elInSet with | intro f hf => 
+    apply mIsModel.left
+    simp [Set.element] 
+    have : f = el := by have hfr := hf.right; simp [applyFact, List.map_id'] at hfr; exact hfr
+    rw [this] at hf
+    exact hf.left
+)⟩ 
+| .succ j => 
+  let prev_hom := inductive_homomorphism kb cs m mIsModel j
+  let trg_ex_dec := Classical.propDecidable (∃ trg : (RTrigger kb.rules), trg.val.ractive (cs.fact_sets j) ∧ trg.val.result ∪ cs.fact_sets j = cs.fact_sets (j + 1))
+  match trg_ex_dec with 
+  | .isFalse n_trg_ex => ⟨prev_hom.val, (by 
+    have sequence_finished := by cases cs.triggers_exist j with
+    | inl _ => contradiction
+    | inr hr => exact hr
+    rw [← sequence_finished.right]
+    exact prev_hom.property
+  )⟩
+  | .isTrue trg_ex =>
+    let trg := Classical.choose trg_ex
+    let ⟨trg_act, trg_res⟩ := Classical.choose_spec trg_ex
+    let trg_on_m : RTrigger kb.rules := {
+      val := {
+        rule := trg.val.rule
+        subs := fun t => prev_hom.val (trg.val.subs t)
+      }
+      property := trg.property
+    }
+
+    have trg_loaded_for_m : trg_on_m.val.loaded m := by 
+      have : trg_on_m.val.loaded (applyFactSet prev_hom (cs.fact_sets j)) := by 
+        apply Trigger.term_mapping_preserves_loadedness
+        exact prev_hom.property.left
+        exact trg_act.left
+      apply Set.subsetTransitive
+      exact ⟨this, prev_hom.property.right⟩
+    have m_models_trg : m.modelsRule trg_on_m.val.rule := by exact mIsModel.right trg.val.rule trg.property 
+    have trg_obsolete_on_m : trg_on_m.val.robsolete m := by 
+      have nactive := m_models_trg trg_on_m.val ⟨rfl, trg_loaded_for_m⟩ 
+      cases Classical.em (trg_on_m.val.robsolete m) with 
+      | inl h => exact h
+      | inr nh => 
+        have : trg_on_m.val.ractive m := ⟨trg_loaded_for_m, nh⟩
+        contradiction
+
+    let subs := Classical.choose trg_obsolete_on_m
+    let hsubs := Classical.choose_spec trg_obsolete_on_m
+
+    let new_h : GroundTermMapping := fun t =>
+      match t_eq : t with 
+      | GroundTerm.const _ => t
+      | GroundTerm.func ft =>
+        let tInChaseKDec := Classical.propDecidable (∃ f, f ∈ (cs.fact_sets j) ∧ t ∈ f.terms.toSet)
+        match tInChaseKDec with 
+        | Decidable.isTrue _ => prev_hom.val t
+        | Decidable.isFalse tNotInChaseK =>
+          let tInResultDec := Classical.propDecidable (∃ f, f ∈ trg.val.result ∧ t ∈ f.terms.toSet)
+          match tInResultDec with 
+          | Decidable.isFalse _ => t
+          | Decidable.isTrue tInResult =>
+            let f := Classical.choose tInResult
+            let ⟨hfl, hfr⟩ := Classical.choose_spec tInResult
+
+            let idx_f := trg.val.idx_of_fact_in_result f hfl
+            let atom_in_head := trg.val.rule.head.get idx_f
+            -- let skolem_atom_in_head := atom_in_head.skolemize trg.val.rule.id trg.val.rule.frontier
+            let idx_t_in_f := f.terms.idx_of t (List.listToSetElementAlsoListElement _ _ hfr)
+            have idx_t_in_f_isLt := idx_t_in_f.isLt
+            have f_is_at_its_idx : f = trg.val.mapped_head.get ⟨idx_f.val, by simp [Trigger.mapped_head, List.length_map, List.length_enum]; exact idx_f.isLt⟩ := by simp [Trigger.idx_of_fact_in_result]; apply List.idx_of_get
+
+            have atom_arity_same_as_fact : f.terms.length = List.length (FunctionFreeAtom.terms atom_in_head) := by 
+                rw [f_is_at_its_idx]
+                unfold Trigger.mapped_head
+                rw [List.get_map]
+                simp
+
+            let term_corresponding_to_t := atom_in_head.terms.get ⟨idx_t_in_f.val, (by 
+              rw [← atom_arity_same_as_fact]
+              exact idx_t_in_f_isLt
+            )⟩
+
+            subs.apply_var_or_const term_corresponding_to_t
+
+    ⟨new_h, (by 
+      constructor 
+      . intro term 
+        split 
+        . simp 
+        . trivial
+      . rw [← trg_res]
+        intro fact fact_in_chase
+        unfold Set.element at fact_in_chase
+
+        cases fact_in_chase with | intro fact' h_fact' =>
+          cases h_fact' with | intro h_fact'_in_chase apply_h_f_and_f'_eq =>
+            cases h_fact'_in_chase with 
+            | inl hl => 
+              let idx_f := trg.val.idx_of_fact_in_result fact' hl
+              have f_is_at_its_idx : fact' = trg.val.mapped_head.get ⟨idx_f.val, by simp [Trigger.mapped_head, List.length_map, List.length_enum]; exact idx_f.isLt⟩ := by simp [Trigger.idx_of_fact_in_result]; apply List.idx_of_get
+
+              rw [← apply_h_f_and_f'_eq]
+              rw [f_is_at_its_idx]
+              unfold applyFact
+
+              apply hsubs.right
+              apply List.existsIndexMeansInToSet
+              exists ⟨idx_f.val, (by simp [SubsTarget.apply, GroundSubstitution.apply_function_free_conj]; apply idx_f.isLt)⟩ 
+              simp [SubsTarget.apply, GroundSubstitution.apply_function_free_conj, List.get_map, GroundSubstitution.apply_function_free_atom, Trigger.mapped_head]
+              rw [List.combine_nested_map]
+              rw [← List.map_eq_map_iff]
+              intro t ht 
+              cases t with 
+              | const ct => simp [VarOrConst.skolemize, GroundSubstitution.apply_term, GroundSubstitution.apply_var_or_const]
+              | var vt => 
+                simp [GroundSubstitution.apply_term, GroundSubstitution.apply_var_or_const]
+                split 
+                case h_1 c h_c_eq =>
+                  have : trg.val.rule.frontier.elem vt := by 
+                    apply Decidable.byContradiction
+                    intro opp
+                    simp [VarOrConst.skolemize, opp] at h_c_eq
+                  rw [hsubs.left vt this]
+                  simp [VarOrConst.skolemize, this]
+                  simp [VarOrConst.skolemize, this] at h_c_eq
+                  rw [h_c_eq]
+                  rw [prev_hom.property.left (GroundTerm.const c)]
+                case h_2 ft h_ft_eq => 
+                  split 
+                  case h_1 _ exis_f _ => 
+                    have vtInHead : ∃ headAtom : FunctionFreeAtom, trg.val.rule.head.elem headAtom ∧ headAtom.terms.elem (VarOrConst.var vt) := by 
+                      exists trg.val.rule.head.get idx_f
+                      simp [List.elem, List.get]
+                      constructor 
+                      . apply List.listToSetElementAlsoListElement
+                        apply List.listGetInToSet
+                      . apply List.listToSetElementAlsoListElement
+                        apply ht
+                    have vtInFrontier : trg.val.rule.frontier.elem vt := by 
+                      apply Decidable.byContradiction
+                      intro vtNotInFrontier
+                      simp at vtNotInFrontier
+
+                      have : trg.val.result ⊆ cs.fact_sets j := by 
+                        apply funcTermForExisVarInChaseMeansTriggerResultOccurs
+                        constructor 
+                        apply vtNotInFrontier
+                        simp [GroundSubstitution.apply_term]
+                        apply exis_f
+
+                      have : trg.val.robsolete (cs.fact_sets j) := by 
+                        let obs_subs := fun v : Variable => trg.val.subs.apply_term (VarOrConst.skolemize (trg.val.rule.id) (trg.val.rule.frontier) (VarOrConst.var v))
+                        exists obs_subs
+                        constructor
+                        . intro v vInFrontier 
+                          simp [obs_subs, GroundSubstitution.apply_term, VarOrConst.skolemize, vInFrontier]
+                        . simp [obs_subs, SubsTarget.apply, GroundSubstitution.apply_function_free_conj]
+                          unfold GroundSubstitution.apply_function_free_atom
+                          intro f' hf'
+                          apply this
+                          unfold Trigger.result
+                          unfold Trigger.mapped_head
+
+                          have : ∀ a : FunctionFreeAtom, (List.map (GroundSubstitution.apply_var_or_const fun v => GroundSubstitution.apply_term trg.val.subs (VarOrConst.skolemize trg.val.rule.id (Rule.frontier trg.val.rule) (VarOrConst.var v))) a.terms) = (List.map (SubsTarget.apply trg.val.subs ∘ VarOrConst.skolemize trg.val.rule.id (Rule.frontier trg.val.rule)) a.terms) := by 
+                            intro a 
+                            induction a.terms with 
+                            | nil => simp [List.map]
+                            | cons head tail ih => 
+                              simp [List.map, ih] 
+                              simp [SubsTarget.apply, GroundSubstitution.apply_term, GroundSubstitution.apply_var_or_const] 
+                              cases head with 
+                              | var v => simp 
+                              | const c => simp [VarOrConst.skolemize]
+
+                          simp [← this]
+                          apply hf'
+
+                      have : ¬ trg.val.robsolete (cs.fact_sets j) := trg_act.right
+
+                      contradiction
+                    rw [hsubs.left]
+                    simp [VarOrConst.skolemize, vtInFrontier]
+                    have : trg.val.rule = trg_on_m.val.rule := by rfl
+                    rw [← this]
+                    apply vtInFrontier
+                  case h_2 _ n_exis_f _ => 
+                    have vtNotInFrontier : ¬ trg.val.rule.frontier.elem vt := by 
+                      intro hcontra
+                      -- TODO: we can show that vt must either be in the database or introduced by a trigger up until step K 
+                      -- which shows the existence of a fact that features the application of subs to the skolemized version 
+                      -- of vt and therefore contradicts n_exis_f
+                      sorry
+                    split 
+                    case h_1 _ n_exis_f' _ => 
+                      apply False.elim 
+                      apply n_exis_f'
+                      exists fact'
+                      constructor 
+                      exact hl 
+                      rw [f_is_at_its_idx]
+
+                      rw [← Trigger.apply_subs_to_atom_at_idx_same_as_fact_at_idx]
+
+                      apply List.existsIndexMeansInToSet
+                      cases (List.inToSetMeansExistsIndex _ _ ht) with | intro term_idx h_term_idx =>
+                        exists ⟨term_idx.val, (by 
+                          rw [← GroundSubstitution.apply_same_length]
+                          rw [← FunctionFreeAtom.skolemize_same_length]
+                          apply term_idx.isLt
+                        )⟩
+                        simp [GroundSubstitution.apply_atom, VarOrConst.skolemize, List.get_map, GroundSubstitution.apply_term, FunctionFreeAtom.skolemize]
+                        rw [← h_term_idx]
+                    case h_2 _ exis_f' _ => 
+                      split
+                      case _ _ chosen_f_hl chosen_f_hr _ =>
+
+                        -- let t := VarOrConst.skolemize trg.val.rule.id (Rule.frontier trg.val.rule) (VarOrConst.var vt)
+                        let t := VarOrConst.var vt
+                        let skolem_t := VarOrConst.skolemize trg.val.rule.id (Rule.frontier trg.val.rule) t
+                        let chosen_f := Classical.choose exis_f'
+
+                        let idx_f := trg.val.idx_of_fact_in_result chosen_f chosen_f_hl
+                        let atom_in_head := trg.val.rule.head.get idx_f
+                        let skolem_atom_in_head := atom_in_head.skolemize trg.val.rule.id trg.val.rule.frontier
+                        let idx_t_in_f := chosen_f.terms.idx_of (trg.val.subs.apply_term skolem_t) (List.listToSetElementAlsoListElement _ _ chosen_f_hr)
+                        have idx_t_in_f_isLt := idx_t_in_f.isLt
+                        have f_is_at_its_idx : chosen_f = trg.val.mapped_head.get ⟨idx_f.val, by simp [Trigger.mapped_head, List.length_map, List.length_enum]; exact idx_f.isLt⟩ := by simp [Trigger.idx_of_fact_in_result]; apply List.idx_of_get
+                        have t_is_at_its_idx : (trg.val.subs.apply_term skolem_t) = chosen_f.terms.get idx_t_in_f := by simp [idx_t_in_f]; apply List.idx_of_get
+
+                        have skolem_atom_in_head_with_subs_is_f : trg.val.subs.apply_atom skolem_atom_in_head = chosen_f := by rw [f_is_at_its_idx]; exact trg.val.apply_subs_to_atom_at_idx_same_as_fact_at_idx idx_f
+
+                        have skolem_atom_arity_same_as_fact : chosen_f.terms.length = List.length skolem_atom_in_head.terms := by 
+                          apply Eq.symm
+                          apply GroundSubstitution.eq_under_subs_means_same_length trg.val.subs
+                          rw [← skolem_atom_in_head_with_subs_is_f]
+
+                        have subs_application_is_injective_for_freshly_introduced_terms : ∀ s, s ∈ skolem_atom_in_head.terms.toSet ∧ trg.val.subs.apply_term skolem_t = trg.val.subs.apply_term s -> skolem_t = s := by 
+                          -- TODO: resolve this by arguing that subs application is basically injective on fresh skolem term
+                          sorry
+
+                        have skolem_t_is_at_its_idx : skolem_t = skolem_atom_in_head.terms.get ⟨idx_t_in_f.val, (by rw[← skolem_atom_arity_same_as_fact]; exact idx_t_in_f_isLt)⟩ := by 
+                          simp [idx_t_in_f]
+
+                          have : skolem_atom_in_head.terms.elem skolem_t := by 
+                            rw [← GroundSubstitution.eq_under_subs_means_elements_are_preserved _ _ _ (skolem_atom_in_head_with_subs_is_f) _ (subs_application_is_injective_for_freshly_introduced_terms)]
+                            apply List.listToSetElementAlsoListElement
+                            apply chosen_f_hr
+                          have : (skolem_atom_in_head.terms.idx_of skolem_t this).val = idx_t_in_f.val := by 
+                            apply Eq.symm
+                            apply GroundSubstitution.eq_under_subs_means_indices_of_elements_are_preserved
+                            apply skolem_atom_in_head_with_subs_is_f
+                            apply subs_application_is_injective_for_freshly_introduced_terms
+
+                          simp [← this]
+                          apply List.idx_of_get
+
+                        let skolem_term_corresponding_to_t := skolem_atom_in_head.terms.get ⟨idx_t_in_f.val, (by 
+                          rw [← skolem_atom_arity_same_as_fact]
+                          exact idx_t_in_f_isLt
+                        )⟩
+
+                        have skolemized_ts_are_equal : skolem_term_corresponding_to_t = skolem_t := by 
+                          rw [skolem_t_is_at_its_idx]
+
+                        have atom_arity_same_as_fact : chosen_f.terms.length = List.length (FunctionFreeAtom.terms atom_in_head) := by 
+                          rw [f_is_at_its_idx]
+                          unfold Trigger.mapped_head
+                          rw [List.get_map]
+                          simp
+
+                        let term_corresponding_to_t := atom_in_head.terms.get ⟨idx_t_in_f.val, (by 
+                          rw [← atom_arity_same_as_fact]
+                          exact idx_t_in_f_isLt
+                        )⟩
+                        
+                        have : VarOrConst.skolemize trg.val.rule.id (Rule.frontier trg.val.rule) term_corresponding_to_t = skolem_term_corresponding_to_t := by simp [FunctionFreeAtom.skolemize, List.get_map]
+
+                        have : term_corresponding_to_t = t := by 
+                          -- TODO: should follow from skolemized_ts_are_equal if we argue that skolemization is injective in the scope of a rule
+                          apply VarOrConst.skolemize_injective trg.val.rule.id (Rule.frontier trg.val.rule)
+                          rw [this]
+                          apply skolemized_ts_are_equal
+
+                        simp [GroundSubstitution.apply_term] at this
+                        rw [this]
+
+            | inr hr => 
+              apply prev_hom.property.right 
+              exists fact'
+              constructor
+              exact hr 
+              unfold applyFact at apply_h_f_and_f'_eq
+              unfold applyFact
+              rw [← apply_h_f_and_f'_eq]
+              simp
+              rw [← List.map_eq_map_iff]
+              intro x hx
+              cases x with 
+              | const xc => simp; apply prev_hom.property.left (GroundTerm.const xc)
+              | func xfunc => 
+                simp 
+                have : ∃ f, f ∈ (cs.fact_sets j) ∧ (GroundTerm.func xfunc) ∈ f.terms.toSet := by exists fact' 
+                split
+                . rfl
+                . contradiction
+    )⟩
+
+theorem inductive_homomorphism_same_on_terms_in_next_step (kb : KnowledgeBase) (cs : ChaseSequence kb) (m : FactSet) (mIsModel : m.modelsKb kb) : ∀ i f t, f ∈ cs.fact_sets i ∧ t ∈ f.terms.toSet -> (inductive_homomorphism kb cs m mIsModel i).val t = (inductive_homomorphism kb cs m mIsModel (Nat.succ i)).val t := by 
+  intro i f t ⟨f_in_step_i, t_is_term_in_f⟩
+  sorry
+
+theorem inductive_homomorphism_same_on_all_following_terms (kb : KnowledgeBase) (cs : ChaseSequence kb) (m : FactSet) (mIsModel : m.modelsKb kb) : ∀ i j f t, f ∈ cs.fact_sets i ∧ t ∈ f.terms.toSet -> (inductive_homomorphism kb cs m mIsModel i).val t = (inductive_homomorphism kb cs m mIsModel (i + j)).val t := by 
+  intro i j f t
+  induction j with 
+  | zero => intros; rfl
+  | succ k ih => 
+    intro h_precondition
+    rw [ih h_precondition]
+    apply inductive_homomorphism_same_on_terms_in_next_step
+    constructor
+    apply chaseSequenceSetIsSubsetOfAllFollowing
+    apply h_precondition.left
+    apply h_precondition.right
+
 theorem chaseResultUnivModelsKb (kb : KnowledgeBase) (cs : ChaseSequence kb) : cs.result.universallyModelsKb kb := by
   constructor
   constructor
+
   -- DB in CS
   simp [FactSet.modelsDb, ChaseSequence.result]
   intro f 
@@ -215,13 +547,14 @@ theorem chaseResultUnivModelsKb (kb : KnowledgeBase) (cs : ChaseSequence kb) : c
   exists 0
   rw [cs.database_first]
   exact h
+  
   -- Rules modelled
   simp [FactSet.modelsRules]
   intro r 
   intro h 
   simp [FactSet.modelsRule]
   intro trg 
-  intro ⟨ trgRule, trgLoaded ⟩
+  intro ⟨ trgRule, _ ⟩
   intro contra 
   cases (trgRActiveForChaseResultMeansRActiveAtSomeIndex kb cs trg contra) with | intro i ractiveI => 
     have notActiveAtSomePoint := cs.fairness ⟨trg, by rw [← trgRule] at h; apply h⟩ i ractiveI 
@@ -238,380 +571,89 @@ theorem chaseResultUnivModelsKb (kb : KnowledgeBase) (cs : ChaseSequence kb) : c
       have obsoleteResult := rObsoletenessSubsetMonotone _ _ _ (And.intro (chaseSequenceSetIsSubsetOfResult kb cs j) obsoleteJ)
       have notObsoleteResult := contra.right 
       contradiction
+  
   -- universality
   intro m mIsModel
-  have inductive_claim : ∀ i : Nat, ∃ h, isHomomorphism h ∧ applyFactSet h (cs.fact_sets i) ⊆ m := by 
-    intro i 
-    induction i 
-    exists id -- is the ID ok here?
-    constructor 
-    unfold isHomomorphism ; intro gt ; cases gt <;> simp
-    rw [cs.database_first]
-    intro el 
-    simp [Set.element]
-    intro elInSet 
-    cases elInSet with | intro f hf => 
-      apply mIsModel.left
-      simp [Set.element] 
-      have : f = el := by have hfr := hf.right; simp [applyFact, List.map_id'] at hfr; exact hfr
-      rw [this] at hf
-      exact hf.left
-    
-    case succ k ih_k => 
-      cases ih_k with | intro h ih_h => 
-        cases cs.triggers_exist k
-        case inr sequence_finished => 
-          exists h 
-          rw [← sequence_finished.right]
-          exact ih_h
-        case inl triggers_exist => 
-          cases triggers_exist with | intro trg h_trg =>
-            let ⟨trg_act, trg_res⟩ := h_trg
-            let trg_on_m : RTrigger kb.rules := {
-              val := {
-                rule := trg.val.rule
-                subs := fun t => h (trg.val.subs t)
-              }
-              property := trg.property
-            }
-            have trg_loaded_for_m : trg_on_m.val.loaded m := by 
-              have : trg_on_m.val.loaded (applyFactSet h (cs.fact_sets k)) := by 
-                apply Trigger.term_mapping_preserves_loadedness
-                exact ih_h.left
-                exact trg_act.left
-              apply Set.subsetTransitive
-              exact ⟨this, ih_h.right⟩
-            have m_models_trg : m.modelsRule trg_on_m.val.rule := by exact mIsModel.right trg.val.rule trg.property 
-            have trg_obsolete_on_m : trg_on_m.val.robsolete m := by 
-              have nactive := m_models_trg trg_on_m.val ⟨rfl, trg_loaded_for_m⟩ 
-              cases Classical.em (trg_on_m.val.robsolete m) with 
-              | inl h => exact h
-              | inr nh => 
-                have : trg_on_m.val.ractive m := ⟨trg_loaded_for_m, nh⟩
-                contradiction
 
-            let subs := Classical.choose trg_obsolete_on_m
-            let hsubs := Classical.choose_spec trg_obsolete_on_m
-              
-            let new_h : GroundTermMapping := fun t =>
-              match t_eq : t with 
-              | GroundTerm.const _ => t
-              | GroundTerm.func ft =>
-                let tInChaseKDec := Classical.propDecidable (∃ f, f ∈ (cs.fact_sets k) ∧ t ∈ f.terms.toSet)
-                match tInChaseKDec with 
-                | Decidable.isTrue _ => h t
-                | Decidable.isFalse tNotInChaseK =>
-                  let tInResultDec := Classical.propDecidable (∃ f, f ∈ trg.val.result ∧ t ∈ f.terms.toSet)
-                  match tInResultDec with 
-                  | Decidable.isFalse _ => t
-                  | Decidable.isTrue tInResult =>
-                    let f := Classical.choose tInResult
-                    let ⟨hfl, hfr⟩ := Classical.choose_spec tInResult
-
-                    let idx_f := trg.val.idx_of_fact_in_result f hfl
-                    let atom_in_head := trg.val.rule.head.get idx_f
-                    -- let skolem_atom_in_head := atom_in_head.skolemize trg.val.rule.id trg.val.rule.frontier
-                    let idx_t_in_f := f.terms.idx_of t (List.listToSetElementAlsoListElement _ _ hfr)
-                    have idx_t_in_f_isLt := idx_t_in_f.isLt
-                    have f_is_at_its_idx : f = trg.val.mapped_head.get ⟨idx_f.val, by simp [Trigger.mapped_head, List.length_map, List.length_enum]; exact idx_f.isLt⟩ := by simp [Trigger.idx_of_fact_in_result]; apply List.idx_of_get
-                    -- have t_is_at_its_idx : t = f.terms.get idx_t_in_f := by simp [idx_t_in_f]; apply List.idx_of_get
-
-                    -- have skolem_atom_in_head_with_subs_is_f : trg.val.subs.apply_atom skolem_atom_in_head = f := by rw [f_is_at_its_idx]; exact trg.val.apply_subs_to_atom_at_idx_same_as_fact_at_idx idx_f
-                    --
-                    -- have skolem_atom_arity_same_as_fact : f.terms.length = List.length skolem_atom_in_head.terms := by 
-                    --   apply Eq.symm
-                    --   apply GroundSubstitution.eq_under_subs_means_same_length trg.val.subs
-                    --   rw [← skolem_atom_in_head_with_subs_is_f]
-
-                    have atom_arity_same_as_fact : f.terms.length = List.length (FunctionFreeAtom.terms atom_in_head) := by 
-                        rw [f_is_at_its_idx]
-                        unfold Trigger.mapped_head
-                        rw [List.get_map]
-                        -- rw [List.get_enum]
-                        simp
-
-                    let term_corresponding_to_t := atom_in_head.terms.get ⟨idx_t_in_f.val, (by 
-                      rw [← atom_arity_same_as_fact]
-                      exact idx_t_in_f_isLt
-                    )⟩
-                    -- have : trg.val.subs.apply_term term_corresponding_to_t = t := by 
-                    --   rw [t_is_at_its_idx]
-                    --   apply GroundSubstitution.eq_under_subs_means_term_is_eq trg.val.subs
-                    --   rw [← skolem_atom_in_head_with_subs_is_f]
-
-                    subs.apply_var_or_const term_corresponding_to_t
-
-            exists new_h
-            constructor 
-            . intro term; cases term with 
-              | const c => simp 
-              | func _ => trivial
-            . rw [← trg_res]
-              intro fact fact_in_chase
-              unfold Set.element at fact_in_chase
-
-              cases fact_in_chase with | intro fact' h_fact' =>
-                cases h_fact' with | intro h_fact'_in_chase apply_h_f_and_f'_eq =>
-                  cases h_fact'_in_chase with 
-                  | inl hl => 
-                    let idx_f := trg.val.idx_of_fact_in_result fact' hl
-                    have f_is_at_its_idx : fact' = trg.val.mapped_head.get ⟨idx_f.val, by simp [Trigger.mapped_head, List.length_map, List.length_enum]; exact idx_f.isLt⟩ := by simp [Trigger.idx_of_fact_in_result]; apply List.idx_of_get
-
-                    rw [← apply_h_f_and_f'_eq]
-                    rw [f_is_at_its_idx]
-                    unfold applyFact
-
-                    apply hsubs.right
-                    apply List.existsIndexMeansInToSet
-                    exists ⟨idx_f.val, (by simp [SubsTarget.apply, GroundSubstitution.apply_function_free_conj]; apply idx_f.isLt)⟩ 
-                    simp [SubsTarget.apply, GroundSubstitution.apply_function_free_conj, List.get_map, GroundSubstitution.apply_function_free_atom, Trigger.mapped_head]
-                    rw [List.combine_nested_map]
-                    rw [← List.map_eq_map_iff]
-                    intro t ht 
-                    cases t with 
-                    | const ct => simp [VarOrConst.skolemize, GroundSubstitution.apply_term, GroundSubstitution.apply_var_or_const]
-                    | var vt => 
-                      simp [GroundSubstitution.apply_term, GroundSubstitution.apply_var_or_const]
-                      split 
-                      case h_1 c h_c_eq =>
-                        have : trg.val.rule.frontier.elem vt := by 
-                          apply Decidable.byContradiction
-                          intro opp
-                          simp [VarOrConst.skolemize, opp] at h_c_eq
-                        rw [hsubs.left vt this]
-                        simp [VarOrConst.skolemize, this]
-                        simp [VarOrConst.skolemize, this] at h_c_eq
-                        rw [h_c_eq]
-                        rw [ih_h.left (GroundTerm.const c)]
-                      case h_2 ft h_ft_eq => 
-                        split 
-                        case h_1 _ exis_f _ => 
-                          have vtInHead : ∃ headAtom : FunctionFreeAtom, trg.val.rule.head.elem headAtom ∧ headAtom.terms.elem (VarOrConst.var vt) := by 
-                            exists trg.val.rule.head.get idx_f
-                            simp [List.elem, List.get]
-                            constructor 
-                            . apply List.listToSetElementAlsoListElement
-                              apply List.listGetInToSet
-                            . apply List.listToSetElementAlsoListElement
-                              apply ht
-                          have vtInFrontier : trg.val.rule.frontier.elem vt := by 
-                            apply Decidable.byContradiction
-                            intro vtNotInFrontier
-                            simp at vtNotInFrontier
-
-                            have : trg.val.result ⊆ cs.fact_sets k := by 
-                              apply funcTermForExisVarInChaseMeansTriggerResultOccurs
-                              constructor 
-                              apply vtNotInFrontier
-                              simp [GroundSubstitution.apply_term]
-                              apply exis_f
-
-                            have : trg.val.robsolete (cs.fact_sets k) := by 
-                              let obs_subs := fun v : Variable => trg.val.subs.apply_term (VarOrConst.skolemize (trg.val.rule.id) (trg.val.rule.frontier) (VarOrConst.var v))
-                              exists obs_subs
-                              constructor
-                              . intro v vInFrontier 
-                                simp [obs_subs, GroundSubstitution.apply_term, VarOrConst.skolemize, vInFrontier]
-                              . simp [obs_subs, SubsTarget.apply, GroundSubstitution.apply_function_free_conj]
-                                unfold GroundSubstitution.apply_function_free_atom
-                                intro f' hf'
-                                apply this
-                                unfold Trigger.result
-                                unfold Trigger.mapped_head
-
-                                have : ∀ a : FunctionFreeAtom, (List.map (GroundSubstitution.apply_var_or_const fun v => GroundSubstitution.apply_term trg.val.subs (VarOrConst.skolemize trg.val.rule.id (Rule.frontier trg.val.rule) (VarOrConst.var v))) a.terms) = (List.map (SubsTarget.apply trg.val.subs ∘ VarOrConst.skolemize trg.val.rule.id (Rule.frontier trg.val.rule)) a.terms) := by 
-                                  intro a 
-                                  induction a.terms with 
-                                  | nil => simp [List.map]
-                                  | cons head tail ih => 
-                                    simp [List.map, ih] 
-                                    simp [SubsTarget.apply, GroundSubstitution.apply_term, GroundSubstitution.apply_var_or_const] 
-                                    cases head with 
-                                    | var v => simp 
-                                    | const c => simp [VarOrConst.skolemize]
-
-                                simp [← this]
-                                apply hf'
-
-                            have : ¬ trg.val.robsolete (cs.fact_sets k) := trg_act.right
-
-                            contradiction
-                          rw [hsubs.left]
-                          simp [VarOrConst.skolemize, vtInFrontier]
-                          have : trg.val.rule = trg_on_m.val.rule := by rfl
-                          rw [← this]
-                          apply vtInFrontier
-                        case h_2 _ n_exis_f _ => 
-                          have vtNotInFrontier : ¬ trg.val.rule.frontier.elem vt := by 
-                            intro hcontra
-                            -- we can show that vt must either be in the database or introduced by a trigger up until step K 
-                            -- which shows the existence of a fact that features the application of subs to the skolemized version 
-                            -- of vt and therefore contradicts n_exis_f
-                            sorry
-                          split 
-                          case h_1 _ n_exis_f' _ => 
-                            apply False.elim 
-                            apply n_exis_f'
-                            exists fact'
-                            constructor 
-                            exact hl 
-                            rw [f_is_at_its_idx]
-
-                            rw [← Trigger.apply_subs_to_atom_at_idx_same_as_fact_at_idx]
-
-                            apply List.existsIndexMeansInToSet
-                            cases (List.inToSetMeansExistsIndex _ _ ht) with | intro term_idx h_term_idx =>
-                              exists ⟨term_idx.val, (by 
-                                rw [← GroundSubstitution.apply_same_length]
-                                rw [← FunctionFreeAtom.skolemize_same_length]
-                                apply term_idx.isLt
-                              )⟩
-                              simp [GroundSubstitution.apply_atom, VarOrConst.skolemize, List.get_map, GroundSubstitution.apply_term, FunctionFreeAtom.skolemize]
-                              rw [← h_term_idx]
-                          case h_2 _ exis_f' _ => 
-                            split
-                            case _ _ chosen_f_hl chosen_f_hr _ =>
-
-                              -- let t := VarOrConst.skolemize trg.val.rule.id (Rule.frontier trg.val.rule) (VarOrConst.var vt)
-                              let t := VarOrConst.var vt
-                              let skolem_t := VarOrConst.skolemize trg.val.rule.id (Rule.frontier trg.val.rule) t
-                              let chosen_f := Classical.choose exis_f'
-
-                              let idx_f := trg.val.idx_of_fact_in_result chosen_f chosen_f_hl
-                              let atom_in_head := trg.val.rule.head.get idx_f
-                              let skolem_atom_in_head := atom_in_head.skolemize trg.val.rule.id trg.val.rule.frontier
-                              let idx_t_in_f := chosen_f.terms.idx_of (trg.val.subs.apply_term skolem_t) (List.listToSetElementAlsoListElement _ _ chosen_f_hr)
-                              have idx_t_in_f_isLt := idx_t_in_f.isLt
-                              have f_is_at_its_idx : chosen_f = trg.val.mapped_head.get ⟨idx_f.val, by simp [Trigger.mapped_head, List.length_map, List.length_enum]; exact idx_f.isLt⟩ := by simp [Trigger.idx_of_fact_in_result]; apply List.idx_of_get
-                              have t_is_at_its_idx : (trg.val.subs.apply_term skolem_t) = chosen_f.terms.get idx_t_in_f := by simp [idx_t_in_f]; apply List.idx_of_get
-
-                              have skolem_atom_in_head_with_subs_is_f : trg.val.subs.apply_atom skolem_atom_in_head = chosen_f := by rw [f_is_at_its_idx]; exact trg.val.apply_subs_to_atom_at_idx_same_as_fact_at_idx idx_f
-
-                              have skolem_atom_arity_same_as_fact : chosen_f.terms.length = List.length skolem_atom_in_head.terms := by 
-                                apply Eq.symm
-                                apply GroundSubstitution.eq_under_subs_means_same_length trg.val.subs
-                                rw [← skolem_atom_in_head_with_subs_is_f]
-
-                              have subs_application_is_injective_for_freshly_introduced_terms : ∀ s, s ∈ skolem_atom_in_head.terms.toSet ∧ trg.val.subs.apply_term skolem_t = trg.val.subs.apply_term s -> skolem_t = s := by 
-                                -- TODO: resolve this by arguing that subs application is basically injective on fresh skolem term
-                                sorry
-
-                              have skolem_t_is_at_its_idx : skolem_t = skolem_atom_in_head.terms.get ⟨idx_t_in_f.val, (by rw[← skolem_atom_arity_same_as_fact]; exact idx_t_in_f_isLt)⟩ := by 
-                                simp [idx_t_in_f]
-
-                                have : skolem_atom_in_head.terms.elem skolem_t := by 
-                                  rw [← GroundSubstitution.eq_under_subs_means_elements_are_preserved _ _ _ (skolem_atom_in_head_with_subs_is_f) _ (subs_application_is_injective_for_freshly_introduced_terms)]
-                                  apply List.listToSetElementAlsoListElement
-                                  apply chosen_f_hr
-                                have : (skolem_atom_in_head.terms.idx_of skolem_t this).val = idx_t_in_f.val := by 
-                                  apply Eq.symm
-                                  apply GroundSubstitution.eq_under_subs_means_indices_of_elements_are_preserved
-                                  apply skolem_atom_in_head_with_subs_is_f
-                                  apply subs_application_is_injective_for_freshly_introduced_terms
-
-                                simp [← this]
-                                apply List.idx_of_get
-
-                              let skolem_term_corresponding_to_t := skolem_atom_in_head.terms.get ⟨idx_t_in_f.val, (by 
-                                rw [← skolem_atom_arity_same_as_fact]
-                                exact idx_t_in_f_isLt
-                              )⟩
-
-                              have skolemized_ts_are_equal : skolem_term_corresponding_to_t = skolem_t := by 
-                                rw [skolem_t_is_at_its_idx]
-
-                              have atom_arity_same_as_fact : chosen_f.terms.length = List.length (FunctionFreeAtom.terms atom_in_head) := by 
-                                rw [f_is_at_its_idx]
-                                unfold Trigger.mapped_head
-                                rw [List.get_map]
-                                simp
-
-                              let term_corresponding_to_t := atom_in_head.terms.get ⟨idx_t_in_f.val, (by 
-                                rw [← atom_arity_same_as_fact]
-                                exact idx_t_in_f_isLt
-                              )⟩
-                              
-                              have : VarOrConst.skolemize trg.val.rule.id (Rule.frontier trg.val.rule) term_corresponding_to_t = skolem_term_corresponding_to_t := by simp [FunctionFreeAtom.skolemize, List.get_map]
-
-                              have : term_corresponding_to_t = t := by 
-                                -- TODO: should follow from skolemized_ts_are_equal if we argue that skolemization is injective in the scope of a rule
-                                apply VarOrConst.skolemize_injective trg.val.rule.id (Rule.frontier trg.val.rule)
-                                rw [this]
-                                apply skolemized_ts_are_equal
-
-                              simp [GroundSubstitution.apply_term] at this
-                              rw [this]
-
-                  | inr hr => 
-                    apply ih_h.right 
-                    exists fact'
-                    constructor
-                    exact hr 
-                    unfold applyFact at apply_h_f_and_f'_eq
-                    unfold applyFact
-                    rw [← apply_h_f_and_f'_eq]
-                    simp
-                    rw [← List.map_eq_map_iff]
-                    intro x hx
-                    cases x with 
-                    | const xc => simp; apply ih_h.left (GroundTerm.const xc)
-                    | func xfunc => 
-                      simp 
-                      have : ∃ f, f ∈ (cs.fact_sets k) ∧ (GroundTerm.func xfunc) ∈ f.terms.toSet := by exists fact' 
-                      split
-                      . rfl
-                      . contradiction
+  let inductive_homomorphism_shortcut := inductive_homomorphism kb cs m mIsModel
 
   let global_h : GroundTermMapping := fun t => 
     let dec := Classical.propDecidable (∃ f, f ∈ cs.result ∧ t ∈ f.terms.toSet)
     match dec with
       | Decidable.isTrue p => 
-        let f := Classical.choose p 
-        let ⟨hfl, hfr⟩ := Classical.choose_spec p
+        let ⟨hfl, _⟩ := Classical.choose_spec p
         let i := Classical.choose hfl
-        let hi := Classical.choose_spec hfl
-        let target_h := Classical.choose (inductive_claim i)
-        target_h t
+        let target_h := inductive_homomorphism_shortcut i
+        target_h.val t
       | Decidable.isFalse _ => t
+
+  have : ∀ i f, f ∈ cs.fact_sets i -> applyFact global_h f = applyFact (inductive_homomorphism_shortcut i).val f := by 
+    intro i f f_in_step_i
+    unfold applyFact
+    simp
+    apply List.map_eq_map_if_functions_eq
+    intro t t_is_term_in_f
+    split 
+    case a.h_2 _ n_ex_f' _ => 
+      -- contradiction
+      apply False.elim 
+      apply n_ex_f' 
+      exists f 
+      constructor 
+      . apply chaseSequenceSetIsSubsetOfResult; apply f_in_step_i
+      . apply t_is_term_in_f
+    case a.h_1 _ ex_f' _ => 
+      split
+      case _ f' t_is_term_in_f' _ => 
+        let j := Classical.choose f'
+        let f'_in_step_j := Classical.choose_spec f'
+        cases Nat.le_total i j with
+        | inl i_le_j => 
+          have j_is_i_plus_k := Nat.le.dest i_le_j 
+          cases j_is_i_plus_k with | intro k hk =>
+            simp at hk
+            rw [← hk]
+            apply Eq.symm
+            apply inductive_homomorphism_same_on_all_following_terms
+            constructor
+            apply f_in_step_i
+            apply t_is_term_in_f
+        | inr j_le_i => 
+          have i_is_j_plus_k := Nat.le.dest j_le_i 
+          cases i_is_j_plus_k with | intro k hk =>
+            rw [← hk]
+            apply inductive_homomorphism_same_on_all_following_terms
+            constructor
+            apply f'_in_step_j
+            apply t_is_term_in_f'
+  
   exists global_h
   constructor
-  intro gt 
-  cases gt with
-    | const c => 
-      simp
-      cases Classical.propDecidable (∃ f, f ∈ ChaseSequence.result cs ∧ GroundTerm.const c ∈ List.toSet f.terms) with 
-        | isTrue p => 
-          simp 
-          let f := Classical.choose p 
-          let ⟨hfl, hfr⟩ := Classical.choose_spec p
-          let i := Classical.choose hfl
-          let hi := Classical.choose_spec hfl
-          let target_h := Classical.choose (inductive_claim i)
-          let target_h_is_hom := (Classical.choose_spec (inductive_claim i)).left
-          simp
-          exact target_h_is_hom (GroundTerm.const c)
-        | isFalse np => simp
-    | _ => simp
+  . intro gt 
+    split 
+    case h_1 _ c => 
+      simp 
+      split 
+      . split 
+        case h_1 hfl _ _ => 
+          let i := Classical.choose hfl 
+          exact (inductive_homomorphism_shortcut i).property.left (GroundTerm.const c)
+      . trivial
+    . trivial
 
-  have : ∀ i f, f ∈ cs.fact_sets i -> applyFact global_h f = applyFact (Classical.choose (inductive_claim i)) f := by 
-    -- TODO: maybe the inductive claim needs to have an additional result telling us that 
-    -- the homomorphisms all agree an previously introduced terms 
-    -- also: probably global_h needs to be changed
-    sorry
-
-  intro f hf
-  unfold ChaseSequence.result at hf
-  unfold Set.element at hf
-  unfold applyFactSet at hf
-  cases hf with | intro e he =>
-    let ⟨hel, her⟩ := he 
-    simp [Set.element] at hel
-    cases hel with | intro n hn =>
-      rw [← her]
-      rw [this n e hn]
-      have : applyFactSet (Classical.choose (inductive_claim n)) (cs.fact_sets n) ⊆ m := (Classical.choose_spec (inductive_claim n)).right
-      unfold Set.subset at this
-      apply this
-      simp [Set.element, applyFactSet]
-      exists e
+  . intro f hf
+    unfold ChaseSequence.result at hf
+    unfold Set.element at hf
+    unfold applyFactSet at hf
+    cases hf with | intro e he =>
+      let ⟨hel, her⟩ := he 
+      simp [Set.element] at hel
+      cases hel with | intro n hn =>
+        rw [← her]
+        rw [this n e hn]
+        have : applyFactSet (inductive_homomorphism_shortcut n).val (cs.fact_sets n) ⊆ m := (inductive_homomorphism_shortcut n).property.right
+        unfold Set.subset at this
+        apply this
+        simp [Set.element, applyFactSet]
+        exists e
 
